src/HeapADT.v
@@ -7,13 +7,9 @@ Require Import
   Here.FromADT
   Here.Heap.
 
-Section HeapADT.
+Module HeapADT (Mem : Memory).
 
-Variable Word8 : Type.
-Variable Zero  : Word8.
-
-Definition MemoryBlock := MemoryBlock Word8.
-Definition HeapSpec    := @HeapSpec Word8.
+Module Import H := Heap Mem.
 
 Lemma empty_fromADT r :
   refine (callCons HeapSpec emptyS) (ret r) -> fromADT HeapSpec r.
@@ -65,7 +61,7 @@ Proof. intros; check method (fromMeth HeapSpec memcpyS r (fst v)). Qed.
 
 Lemma memset_fromADT r :
   fromADT HeapSpec r
-    -> forall (addr : N) (len : N) (w : Word8) v,
+    -> forall (addr : N) (len : N) (w : Mem.Word8) v,
          refine (callMeth HeapSpec memsetS r addr len w) (ret v)
     -> fromADT HeapSpec (fst v).
 Proof. intros; check method (fromMeth HeapSpec memsetS r (fst v)). Qed.
@@ -80,20 +76,20 @@ Proof.
   hone representation using
     (fun (or : Rep HeapSpec)
          (nr : { r : Rep HeapSpec | fromADT HeapSpec r }) => or = ` nr).
-  resolve_constructor (@empty Word8) empty_fromADT.
-  resolve_method r_n (@alloc Word8 (` r_n) d)
+  resolve_constructor empty empty_fromADT.
+  resolve_method r_n (alloc (` r_n) d)
                      (@alloc_fromADT _ (proj2_sig r_n) d).
-  resolve_method r_n (@free Word8 (` r_n) d)
+  resolve_method r_n (free (` r_n) d)
                      (@free_fromADT _ (proj2_sig r_n) d).
-  resolve_method r_n (@realloc Word8 (` r_n) d d0)
+  resolve_method r_n (realloc (` r_n) d d0)
                      (@realloc_fromADT _ (proj2_sig r_n) d d0).
-  resolve_method r_n (@peek Word8 (` r_n) d)
+  resolve_method r_n (peek (` r_n) d)
                      (@peek_fromADT _ (proj2_sig r_n) d).
-  resolve_method r_n (@poke Word8 (` r_n) d d0)
+  resolve_method r_n (poke (` r_n) d d0)
                      (@poke_fromADT _ (proj2_sig r_n) d d0).
-  resolve_method r_n (@memcpy Word8 (` r_n) d d0 d1)
+  resolve_method r_n (memcpy (` r_n) d d0 d1)
                      (@memcpy_fromADT _ (proj2_sig r_n) d d0 d1).
-  resolve_method r_n (@memset Word8 (` r_n) d d0 d1)
+  resolve_method r_n (memset (` r_n) d d0 d1)
                      (@memset_fromADT _ (proj2_sig r_n) d d0 d1).
   apply reflexivityT.
 Defined.
