src/LibExt.v
@@ -1,7 +1,3 @@
-Require Import Coq.Sets.Ensembles.
-
-Require Import Here.Same_set.
-
 (** Basic definitions added to the standard library. *)
 
 Ltac inv H := inversion H; subst; clear H.
@@ -12,302 +8,117 @@ Definition first {A B C} (f : A -> C) (p : A * B) : C * B :=
 Definition second {A B C} (f : B -> C) (p : A * B) : A * C :=
   (fst p, f (snd p)).
 
-CoInductive stream (A : Type) := scons : A -> stream A -> stream A.
+Require Import
+  Coq.Sets.Ensembles
+  Here.Same_set.
 
-CoFixpoint series (n : nat) : stream nat := scons n (series (S n)).
+Definition Map_set {A B} (f : A -> B) (r : Ensemble A) : Ensemble B :=
+  fun b => exists a : A, In _ r a /\ b = f a.
 
-Fixpoint zip {A B} (xs : stream A) (ys : list B) : list (A * B) :=
-  match xs with
-  | scons x xs =>
-    match ys with
-    | nil => nil
-    | cons y ys => (x, y) :: zip xs ys
-    end
-  end.
-
-Require Import Coq.Lists.List.
-
-Lemma In_zip_series : forall A (x : A) xs n i, n <= i
-  -> List.In (S i, x) (zip (series n) xs)
-  -> exists y, In (i, y) (zip (series n) xs).
+Lemma Map_set_left_identity {A} (r : Ensemble A) : Same_set A r (Map_set id r).
 Proof.
-  Require Import Omega.
-  intros.
-  generalize dependent n.
-  induction xs; intros.
-    inversion H0.
-  simpl in H0.
-  destruct H0.
-    inv H0.
-    abstract omega.
-  simpl.
-  specialize (IHxs (S n)).
-  destruct (Peano_dec.eq_nat_dec n i).
-    exists a.
-    subst.
-    left; reflexivity.
-  assert (not_really_le : forall n i, n <= i -> n <> i -> S n <= i)
-    by (intros; abstract omega).
-  specialize (IHxs (not_really_le _ _ H n0) H0).
-  destruct IHxs.
-  exists x0.
-  right.
-  exact H1.
-Qed.
-
-Lemma In_ascending : forall A (x : A) xs n m,
-  n < m -> ~ In (n, x) (zip (series m) xs).
-Proof.
-  unfold not.
-  induction xs; simpl; intros.
-    contradiction.
-  destruct H0.
-    inv H0.
-    firstorder.
-  apply IHxs with (n:=n) (m:=S m).
-    omega.
-  assumption.
-Qed.
-
-Lemma In_zip_at_index : forall i n A (x y : A) xs,
-  In (i, x) (zip (series n) xs) -> In (i, y) (zip (series n) xs) -> x = y.
-Proof.
-  intros.
-  generalize dependent n.
-  induction xs; simpl; intros.
-    contradiction.
-  destruct H, H0.
-  + inv H; inv H0; reflexivity.
-  + inv H.
-    apply In_ascending in H0; [contradiction|omega].
-  + inv H0.
-    apply In_ascending in H; [contradiction|omega].
-  + apply (IHxs (S n)); trivial.
-Qed.
-
-Lemma pred_S_S : forall n i, Init.Nat.pred n = S i -> n = S (S i).
-Proof. intros; omega. Qed.
-
-Require Import Coq.Arith.Arith.
-
-Program Fixpoint nth_safe
-        {A : Type} (n : nat) (l : list A) : is_true (n <? length l) -> A :=
-  match l as l0 return is_true (n <? length l0) -> A with
-  | nil => fun _ => False_rect _ _
-  | cons x xs =>
-    match n as n0 return is_true (n0 <? length (x :: xs)) -> A with
-    | O => fun _ => x
-    | S n => @nth_safe A n xs
-    end
-  end.
-
-Arguments nth_safe {A} n l _.
-
-Lemma has_Some : forall A B (a : option A) (b : B),
-  a <> None -> exists b, a = Some b.
-Proof.
-  intros.
-  destruct a.
-    exists a; reflexivity.
+  unfold Map_set; split; intros.
+    eexists; intuition.
+    assumption.
+  intros ??.
+  do 2 destruct H.
+  unfold id in H0.
   congruence.
 Qed.
 
-Require Export
-  Coq.Sets.Constructive_sets
-  Coq.Sets.Powerset_facts.
-
-Require Import Fiat.ADT.
-
-Ltac single_reduction :=
-  match goal with
-  | [ |- Strict_Included _ _ _ ] => constructor
-  | [ |- Included _ _ _ ] =>
-    let x := fresh "x" in
-    let Hx := fresh "Hx" in
-    intros x Hx
-  | [ H : _ /\ _ |- _ ] => destruct H
-  | [ |- _ /\ _ ] => split
-  | [ H : _ * _ |- _ ] => destruct H
-  | [ |- _ * _ ] => split
-  | [ H : Ensembles.In _ _ _ |- _ ] => inv H
-  | [ H : Ensembles.In _ _ _ |- _ ] => rewrite H in *
-  | [ |- Ensembles.In _ _ _ ] => constructor
-  | [ |- Ensembles.In _ (Bind _ (fun x => ret _)) _ ] => eexists
-  | [ |- Ensembles.In _ _ _ ] => eexists
-  | [ H : forall x : ?T, Some ?X = Some x -> _ |- _ ] =>
-    specialize (H X eq_refl)
-  | [ |- ret ?C ↝ ?V -> _ ] =>
-    let H := fresh "H" in intro H; apply Return_inv in H; simpl in H; inv H
-  | [ |- Bind ?C ?F ↝ ?V -> _ ] =>
-    let H := fresh "H" in intro H; apply Bind_inv in H; simpl in H; inv H
-  | [ |- Pick ?S ↝ ?V -> _ ] =>
-    let H := fresh "H" in intro H; apply Pick_inv in H; simpl in H; inv H
-  | [ H : ret ?C ↝ ?V     |- _ ] => apply Return_inv in H
-  | [ H : Bind ?C ?F ↝ ?V |- _ ] => apply Bind_inv in H
-  | [ H : Pick ?S ↝ ?V    |- _ ] => apply Pick_inv in H
-  | [ |- ret ?C ↝ ?V ]           => apply ReturnComputes
-  | [ |- Bind ?C ?F ↝ ?V ]       => apply BindComputes
-  | [ |- Pick ?S ↝ ?V ]          => apply PickComputes
-  | [ |- context [If_Opt_Then_Else ?V ?T ?E] ] => destruct V
-  (* | [ |- context [IfDec_Then_Else ?P ?T ?E] ]  => unfold IfDec_Then_Else *)
-  end.
-
-Ltac simplify_ensembles :=
-  repeat (single_reduction; simpl; destruct_ex);
-  try solve [ intuition | constructor ].
-
-Definition Ensemble_map {A B} (f : A -> B) (x : Comp A) : Comp B :=
-  v <- x; ret (f v).
-  (* fun b => exists a, Ensembles.In _ x a /\ b = f a. *)
-
-Lemma refine_ret_Same_set : forall (A : Type) (a : A) (b : Comp A),
-  Same_set _ b (ret a) -> refine (ret a) b.
+Lemma Map_set_right_identity {A} (r : Ensemble A) : Same_set A (Map_set id r) r.
 Proof.
-  intros.
-  rewrite H.
-  reflexivity.
+  unfold Map_set; split; intros.
+    intros ??.
+    do 2 destruct H.
+    unfold id in H0.
+    congruence.
+  eexists; intuition.
+  assumption.
 Qed.
 
-Lemma Same_set_map : forall A B (f : A -> B) x,
-  Same_set _ (fun b => exists a, Ensembles.In _ x a /\ b = f a)
-             (v <- x; ret (f v)).
+Lemma Map_set_composition {A B C} (r : Ensemble A) :
+  forall (f : B -> C) (g : A -> B),
+   Same_set C (Map_set (fun x => f (g x)) r) (Map_set f (Map_set g r)).
 Proof.
-  intros.
-  split; intros v H.
-    inv H.
-    destruct H0.
-    subst.
-    exists x0.
-    split.
-      exact H.
-    constructor.
-  inv H.
-  destruct H0.
-  inv H0.
-  exists x0.
-  split.
-    exact H.
-  reflexivity.
+  unfold Map_set; split; intros; intros ??.
+    do 2 destruct H; subst.
+    exists (g x0); simpl in *.
+    split; trivial.
+    exists x0; simpl.
+    intuition.
+  do 2 destruct H; subst.
+  do 2 destruct H; simpl in *; subst.
+  exists x; simpl in *.
+  intuition.
 Qed.
 
-Lemma Same_set_ret : forall A (X Y : Ensemble A),
-  Same_set A X Y -> Same_set (Ensemble A) (ret X) (ret Y).
+Definition Product {T U} (X : Ensemble T) (Y : Ensemble U) : Ensemble (T * U) :=
+  fun p => In T X (fst p) /\ In U Y (snd p).
+
+Lemma Product_Add_left : forall T U (X : Ensemble T) (Y : Ensemble U) x,
+  Same_set _ (Product (Add T X x) Y)
+             (Union _ (Product (Singleton _ x) Y) (Product X Y)).
 Proof.
-  intros.
+  unfold Product; split; intros;
+  intros ??; unfold Ensembles.In in *;
+  destruct H;
+  destruct x0; simpl in *;
   destruct H.
-  split; intros z H1;
-  inversion H1; subst; clear H1;
-  apply Singleton_intro;
-  apply Extensionality_Ensembles;
-  split; intros z' H1';
-  try apply H0, H1';
-  apply H, H1'.
+  - right; constructor; simpl; auto.
+  - left; constructor; simpl; auto.
+  - simpl in *; intuition; right; intuition.
+  - simpl in *; intuition; left; intuition.
 Qed.
 
-Add Parametric Morphism {A B} : (@Ensemble_map A B)
-  with signature (pointwise_relation _ eq ==> Same_set A ==> Same_set B)
-    as Ensemble_map_Same_set.
+Lemma Product_Add_right : forall T (X : Ensemble T) U (Y : Ensemble U) y,
+  Same_set _ (Product X (Add U Y y))
+             (Union _ (Product X Y) (Product X (Singleton _ y))).
 Proof.
-  unfold Ensemble_map, pointwise_relation; intros.
-  rewrite H0.
-  f_equiv.
-  unfold pointwise_relation; intros.
-  rewrite H.
-  reflexivity.
+  unfold Product; split; intros;
+  intros ??; unfold Ensembles.In in *;
+  destruct H;
+  destruct x; simpl in *.
+  - destruct H0.
+    + left; constructor; simpl; auto.
+    + right; constructor; simpl; auto.
+  - destruct H. intuition; left; intuition.
+  - destruct H. intuition; right; intuition.
 Qed.
 
-Lemma Ensemble_map_id : forall A (xs : Ensemble A),
-  Same_set _ (Ensemble_map id xs) xs.
+Lemma Product_Empty_set_left : forall T U (X : Ensemble U),
+  Same_set _ (Product (Empty_set T) X) (Empty_set (T * U)).
 Proof.
-  intros.
-  autorewrite with monad laws.
-  reflexivity.
+  unfold Product; split; intros;
+  intros ??; unfold Ensembles.In in *.
+  destruct H;
+  destruct x; simpl in *;
+  destruct H.
+  destruct H.
 Qed.
 
-Lemma Ensemble_map_comp : forall A B C xs (f : B -> C) (g : A -> B),
-  Same_set _ (Ensemble_map f (Ensemble_map g xs))
-             (Ensemble_map (fun x => f (g x)) xs).
+Lemma Product_Empty_set_right : forall T (X : Ensemble T) U,
+  Same_set _ (Product X (Empty_set U)) (Empty_set (T * U)).
 Proof.
-  intros.
-  autorewrite with monad laws.
-  reflexivity.
+  unfold Product; split; intros;
+  intros ??; unfold Ensembles.In in *.
+  destruct H;
+  destruct x; simpl in *.
+  destruct H0.
+  destruct H.
 Qed.
 
-Lemma Ensemble_map_Empty_set : forall A B f,
-  Same_set _ (Ensemble_map f (Empty_set A)) (Empty_set B).
+Lemma Product_Singleton_Singleton : forall T U x y,
+  Same_set _ (Product (Singleton T x) (Singleton U y))
+             (Singleton (T * U) (x, y)).
 Proof.
-  unfold Ensemble_map; intros.
-  split; intros x H; simplify_ensembles.
-Qed.
-
-Lemma Ensemble_Add_Subtract : forall A xs x,
-  ~ Ensembles.In A xs x
-    -> Same_set _ (Ensembles.Subtract A (Ensembles.Add A xs x) x) xs.
-Proof.
-  unfold Ensembles.Subtract, Ensembles.Add, Ensembles.Setminus; intros.
-  constructor; intros y H0; simplify_ensembles.
-  unfold not; intros; simplify_ensembles.
-Qed.
-
-Lemma Ensemble_Add_In : forall A xs x,
-  Ensembles.In A (Ensembles.Add A xs x) x.
-Proof. intros; apply Union_intror; constructor. Qed.
-
-Lemma Ensemble_not_In_inv : forall A a b c d,
-  ~ Ensembles.In (nat * A) (Singleton (nat * A) (a, b)) (c, d)
-    -> (a = c -> b <> d) \/ (b = d -> a <> c).
-Proof.
-  intros.
-  destruct (Peano_dec.eq_nat_dec a c); subst.
-    right.
-    intros.
-    subst.
-    contradiction H.
+  unfold Product; split; intros;
+  intros ??; unfold Ensembles.In in *;
+  destruct H.
+    inversion H; subst; clear H.
+    inversion H0; subst; clear H0.
+    rewrite <- surjective_pairing.
     constructor.
-  left.
-  intros.
-  contradiction.
-Qed.
-
-Lemma Ensemble_fst_eq_inv : forall A a b d,
-  ~ Ensembles.In (nat * A) (Singleton (nat * A) (a, b)) (a, d)
-    -> b <> d.
-Proof.
-  intros.
-  intro H1.
-  subst.
-  contradiction H.
-  constructor.
-Qed.
-
-Ltac In_contradiction IHfromADT :=
-  match goal with
-    | [ H1 : ?X <> ?Y,
-        H2 : Ensembles.In (nat * ?A) ?R (?I, ?X),
-        H3 : Ensembles.In (nat * ?A) ?R (?I, ?Y)
-      |- False ] =>
-      apply (IHfromADT Y X) in H2; trivial; contradiction
-  end.
-
-Require Import Fiat.ADTNotation.
-
-Definition lookupMethod
-           (sig : DecoratedADTSig)
-           (idxMap : BoundedIndex (MethodNames sig) -> MethodIndex sig)
-           (idx : BoundedIndex (MethodNames sig)) : MethodIndex sig :=
-  idxMap idx.
-
-Definition getADTSig {sig : DecoratedADTSig} : ADT sig -> DecoratedADTSig :=
-  fun _ => sig.
-
-Definition get_fin {A : Type} {n : nat} {Bound : Vector.t A n}
-                   (idx : BoundedIndex Bound) :=
-  ibound (indexb idx).
-
-Lemma refine_comp_to_pick : forall A (c : Comp A),
-  refine c { x : A | c ↝ x }.
-Proof.
-  intros ????.
-  apply Pick_inv in H.
-  exact H.
+  simpl.
+  intuition.
 Qed.
