src/DefineAbsR.v
@@ -1,0 +1,196 @@
+Require Import
+  Here.LibExt
+  Here.Nomega
+  Here.FMapExt
+  Here.FunMaps
+  Here.TupleEnsembles
+  Coq.FSets.FMapFacts
+  Coq.Structures.DecidableTypeEx.
+
+Generalizable All Variables.
+
+Module Define_AbsR (M : WSfun N_as_DT).
+
+Module F := WFacts_fun N_as_DT M.
+Module Import X := FMapExt N_as_DT M.
+Module Import U := FunMaps N_as_DT M.
+
+Lemma find_define : forall Word8 addr len pos v w m,
+  (IfDec within addr len pos
+   Then v = w
+   Else M.MapsTo pos v m)
+    -> M.MapsTo pos v (N.peano_rect (fun _ => M.t Word8) m
+                                    (fun i => M.add (addr + i)%N w) len).
+Proof.
+  intros.
+  decisions; subst.
+    apply Bool.andb_true_iff in Heqe.
+    destruct Heqe.
+    undecide.
+    induction len using N.peano_ind; simpl in *.
+      rewrite N.add_0_r in H0.
+      nomega.
+    rewrite N.peano_rect_succ.
+    destruct (N.eq_dec pos (addr + len)); subst.
+      intuition.
+    apply F.add_mapsto_iff.
+    right; split; trivial.
+      apply not_eq_sym; assumption.
+    rewrite N.add_succ_r in H0.
+    apply N.lt_succ_r in H0.
+    pose proof (proj2 (N.le_neq pos (addr + len)) (conj H0 n)).
+    apply IHlen; assumption.
+  apply Bool.andb_false_iff in Heqe.
+  destruct Heqe; undecide;
+  induction len using N.peano_ind; simpl in *; auto;
+  rewrite N.peano_rect_succ.
+    simplify_maps.
+    right; split; trivial.
+    unfold not; intros; subst.
+    rewrite <- (N.add_0_r addr) in H0 at 2.
+    apply N.add_lt_cases in H0.
+    destruct H0.
+      nomega.
+    contradiction (N.nlt_0_r len).
+  rewrite N.add_succ_r in H0.
+  simplify_maps.
+  right; split.
+    unfold not; intros; subst.
+    apply N.le_succ_l in H0.
+    nomega.
+  apply IHlen.
+  apply N.le_succ_l in H0.
+  nomega.
+Qed.
+
+Lemma Nle_ne_succ : forall n m,
+  n <> m -> n < N.succ m -> n < m.
+Proof.
+  intros.
+  apply N.le_succ_l in H0.
+  apply N.succ_le_mono in H0.
+  apply N.le_neq; intuition.
+Qed.
+
+Lemma find_define_inv : forall Word8 addr len pos v w m,
+  M.MapsTo pos v (N.peano_rect (fun _ => M.t Word8) m
+                               (fun i => M.add (addr + i)%N w) len)
+    -> IfDec within addr len pos
+       Then v = w
+       Else M.MapsTo pos v m.
+Proof.
+  intros.
+  induction len using N.peano_ind; simpl in *;
+  decisions; auto.
+  - apply Bool.andb_true_iff in Heqe;
+    destruct Heqe; undecide.
+    rewrite N.add_0_r in H1.
+    nomega.
+  - rewrite N.peano_rect_succ in H.
+    simplify_maps; auto.
+  - rewrite N.peano_rect_succ in H.
+    simplify_maps; auto.
+      nomega.
+    apply Bool.andb_true_iff in Heqe;
+    destruct Heqe; undecide.
+    apply Bool.andb_false_iff in Heqe0;
+    destruct Heqe0; undecide.
+      nomega.
+    intuition; subst.
+    rewrite N.add_succ_r in H1.
+    apply N.le_succ_l in H1.
+    nomega.
+  - rewrite N.peano_rect_succ in H.
+    simplify_maps; auto.
+    intuition.
+    apply Bool.andb_true_iff in Heqe0;
+    destruct Heqe0; undecide.
+    apply Bool.andb_false_iff in Heqe;
+    destruct Heqe; undecide.
+      nomega.
+    rewrite N.add_succ_r in H1.
+    apply not_eq_sym in H3.
+    pose proof (Nle_ne_succ H3 H1).
+    nomega.
+  - rewrite N.peano_rect_succ in H.
+    simplify_maps; auto.
+    intuition.
+    apply Bool.andb_false_iff in Heqe0;
+    destruct Heqe0; undecide;
+    apply Bool.andb_false_iff in Heqe;
+    destruct Heqe; undecide.
+    + rewrite <- N.add_0_r in H0.
+      apply N.add_lt_cases in H0.
+      destruct H0.
+        nomega.
+      contradiction (N.nlt_0_r len).
+    + rewrite <- N.add_0_r in H.
+      apply N.add_lt_cases in H.
+      destruct H.
+        nomega.
+      contradiction (N.nlt_0_r len).
+    + rewrite <- N.add_0_r in H0.
+      apply N.add_lt_cases in H0.
+      destruct H0.
+        nomega.
+      contradiction (N.nlt_0_r len).
+    + rewrite N.add_succ_r in H.
+      apply N.le_succ_l in H.
+      nomega.
+Qed.
+
+Lemma Define_Map_AbsR : forall Word8 x y b len w,
+  Map_AbsR eq x y
+    -> Map_AbsR eq (Define (within b len) w x)
+                (N.peano_rect (fun _ => M.t Word8) y
+                              (fun i => M.add (b + i)%N w) len).
+Proof.
+  intros.
+  relational_maps.
+  - teardown.
+    destruct H0, H0; [inv H1|];
+    exists blk; intuition;
+    apply find_define;
+    unfold IfDec_Then_Else; simpl.
+      apply within_reflect in H0.
+      rewrite H0; reflexivity.
+    apply not_within_reflect in H0.
+    rewrite H0.
+    apply H.
+    exists blk; intuition.
+  - reduction.
+    apply find_define_inv in H0.
+    decisions; auto; subst.
+      left.
+      apply within_reflect in Heqe.
+      intuition.
+    right.
+    apply not_within_reflect in Heqe.
+    apply H in H0.
+    destruct H0, H0; subst.
+    intuition.
+  - reduction.
+    apply find_define_inv in H0.
+    decisions; auto; subst.
+      apply within_reflect in Heqe.
+      exists w; intuition.
+      teardown.
+      left; intuition.
+    apply not_within_reflect in Heqe.
+    apply H in H0.
+    destruct H0, H0; subst.
+    exists cblk; intuition.
+    teardown.
+    right; intuition.
+  - repeat teardown; subst; [inv H2|];
+    apply find_define;
+    unfold IfDec_Then_Else; simpl.
+      apply within_reflect in H0.
+      rewrite H0; reflexivity.
+    apply not_within_reflect in H0.
+    rewrite H0.
+    apply H.
+    exists cblk; intuition.
+Qed.
+
+End Define_AbsR.
