src/MemoryBlockC.v
@@ -1,0 +1,151 @@
+Require Import
+  Here.Nomega
+  Here.TupleEnsembles
+  Here.FunMaps
+  Here.Relations
+  Here.Heap
+  Coq.FSets.FMapAVL
+  Coq.FSets.FMapFacts
+  Coq.Structures.DecidableTypeEx
+  Coq.Structures.OrderedTypeEx.
+
+Module MemoryBlockC (Mem : Memory).
+
+Module Import H := Heap Mem.
+Module Import M := FMapAVL.Make(N_as_OT).
+Module Import U := FunMaps N_as_DT M.
+
+Module P := WProperties_fun N_as_DT M.
+Module F := P.F.
+
+Definition MemoryBlock_Same (x y : MemoryBlock) : Prop :=
+  memSize x = memSize y /\ Same (memData x) (memData y).
+
+Global Program Instance MemoryBlock_Proper :
+  Proper (eq ==> @Same _ _ ==> MemoryBlock_Same) Build_MemoryBlock.
+Obligation 1. relational; split; simpl; subst; auto. Qed.
+
+Record MemoryBlockC := {
+  memCSize : N;
+  memCData : M.t Mem.Word8
+}.
+
+Definition MemoryBlockC_Equal (x y : MemoryBlockC) : Prop :=
+  memCSize x = memCSize y /\ M.Equal (memCData x) (memCData y).
+
+Global Program Instance MemoryBlockC_Proper :
+  Proper (eq ==> @M.Equal _ ==> MemoryBlockC_Equal) Build_MemoryBlockC.
+Obligation 1. relational; split; simpl; subst; auto. Qed.
+
+Definition MemoryBlock_AbsR (o : MemoryBlock) (n : MemoryBlockC) : Prop :=
+  memSize o = memCSize n /\ Map_AbsR eq (memData o) (memCData n).
+
+Open Scope lsignature_scope.
+
+Global Program Instance MemoryBlock_AbsR_AbsR :
+  Build_MemoryBlock [R eq ==> Map_AbsR eq ==> MemoryBlock_AbsR]
+  Build_MemoryBlockC.
+Obligation 1. relational; split; simpl; subst; auto. Qed.
+
+Global Program Instance MemoryBlock_AbsR_Proper :
+  Proper (MemoryBlock_Same ==> MemoryBlockC_Equal ==> iff) MemoryBlock_AbsR.
+Obligation 1.
+  relational; destruct H, H0, H1.
+  - split; intros.
+      congruence.
+    split; intros; subst;
+    split; intros.
+    + rewrite <- H2 in H5.
+      apply H4 in H5; trivial.
+      setoid_rewrite H3 in H5.
+      trivial.
+    + rewrite <- H2.
+      apply H4; trivial.
+      setoid_rewrite H3.
+      trivial.
+    + rewrite <- H3 in H5.
+      apply H4 in H5; trivial.
+      setoid_rewrite H2 in H5.
+      trivial.
+    + rewrite <- H3.
+      apply H4; trivial.
+      setoid_rewrite <- H2 in H5.
+      trivial.
+  - split; intros.
+      congruence.
+    split; intros; subst;
+    split; intros.
+    + rewrite H2 in H5.
+      apply H4 in H5; trivial.
+      setoid_rewrite <- H3 in H5.
+      trivial.
+    + rewrite H2.
+      apply H4; trivial.
+      setoid_rewrite <- H3.
+      trivial.
+    + rewrite H3 in H5.
+      apply H4 in H5; trivial.
+      setoid_rewrite <- H2 in H5.
+      trivial.
+    + rewrite H3.
+      apply H4; trivial.
+      setoid_rewrite H2 in H5.
+      trivial.
+Qed.
+
+Corollary MemoryBlock_AbsR_impl : forall s s' d d',
+    s = s' -> Map_AbsR eq d d' ->
+    MemoryBlock_AbsR {| memSize  := s;  memData  := d |}
+                     {| memCSize := s'; memCData := d' |}.
+Proof. intros; subst; split; intros; trivial. Qed.
+
+Corollary Empty_MemoryBlock_AbsR : forall n,
+  MemoryBlock_AbsR {| memSize  := n; memData  := TupleEnsembles.Empty |}
+                   {| memCSize := n; memCData := M.empty Mem.Word8 |}.
+Proof.
+  split; trivial; simpl; intros; apply Empty_Map_AbsR. Qed.
+
+(* [M.Equal] maps are not necessary identical -- for example, there is no
+   ordering requirement -- but for the purposes of proof, they are at least
+   extensionally equal. *)
+Axiom Extensionality_FMap : forall (elt : Type) (A B : M.t elt),
+  M.Equal (elt:=elt) A B -> A = B.
+
+Lemma MemoryBlock_AbsR_FunctionalRelation :
+  FunctionalRelation MemoryBlock_AbsR.
+Proof.
+  intros ?????.
+  destruct H, H0, x, y, z; simpl in *.
+  subst; f_equal.
+  apply Extensionality_FMap.
+  apply F.Equal_mapsto_iff; split; intros.
+    apply H2, H1; trivial.
+  apply H1, H2; trivial.
+Qed.
+
+Lemma MemoryBlock_AbsR_InjectiveRelation :
+  InjectiveRelation MemoryBlock_AbsR.
+Proof.
+  intros ?????.
+  destruct H, H0, x, y, z; simpl in *.
+  subst; f_equal.
+  apply Extensionality_Ensembles.
+  split; intros;
+  intros ??; destruct x.
+    apply H2, H1; trivial.
+  apply H1, H2; trivial.
+Qed.
+
+Lemma eq_FunctionalRelation : forall A, FunctionalRelation (A:=A) (B:=A) eq.
+Proof. intros ??????; subst; reflexivity. Qed.
+
+Lemma eq_InjectiveRelation : forall A,
+  InjectiveRelation (A:=A) (B:=A) eq.
+Proof. intros ??????; subst; reflexivity. Qed.
+
+Hint Resolve MemoryBlock_AbsR_FunctionalRelation.
+Hint Resolve MemoryBlock_AbsR_InjectiveRelation.
+Hint Resolve eq_FunctionalRelation.
+Hint Resolve eq_InjectiveRelation.
+
+End MemoryBlockC.
